src/michocoq/macros.v
@@ -26,7 +26,8 @@ Section macros.
   Context {self_type : self_info}.
 
 Definition CMPop (a : comparable_type) S (op : instruction self_type Datatypes.false (int ::: S) (bool ::: S))
-           : instruction self_type Datatypes.false (a ::: a ::: S) (bool ::: S) := COMPARE ;; op.
+  : instruction self_type Datatypes.false (a ::: a ::: S) (bool ::: S) :=
+  Instruction_seq { COMPARE; op }.
 
 Definition CMPEQ {a S} := CMPop a S EQ.
 Definition CMPNEQ {a S} := CMPop a S NEQ.
@@ -35,10 +36,15 @@ Definition CMPGT {a S} := CMPop a S GT.
 Definition CMPLE {a S} := CMPop a S LE.
 Definition CMPGE {a S} := CMPop a S GE.
 
+Definition wrap_IF {SA SB tffa tffb} (bt : instruction_seq self_type tffa SA SB) (bf : instruction_seq self_type tffb SA SB)
+  : instruction_seq self_type (tffa && tffb)%bool (bool ::: SA) SB :=
+  instruction_wrap (IF_ IF_bool bt bf).
+
 Definition IFop SA SB tffa tffb
-           (bt : instruction self_type tffa SA SB) (bf : instruction self_type tffb SA SB)
-           (op : instruction self_type Datatypes.false (int ::: SA) (bool ::: SA)) :=
-  op ;; IF bt bf.
+           (bt : instruction_seq self_type tffa SA SB) (bf : instruction_seq self_type tffb SA SB)
+           (op : instruction self_type Datatypes.false (int ::: SA) (bool ::: SA))
+  : instruction self_type (tffa && tffb)%bool (int ::: SA) SB :=
+  Instruction_seq (op ;; wrap_IF bt bf).
 
 Definition IFEQ {SA SB tffa tffb} bt bf := IFop SA SB tffa tffb bt bf EQ.
 Definition IFNEQ {SA SB tffa tffb} bt bf := IFop SA SB tffa tffb bt bf NEQ.
@@ -48,10 +54,10 @@ Definition IFLE {SA SB tffa tffb} bt bf := IFop SA SB tffa tffb bt bf LE.
 Definition IFGE {SA SB tffa tffb} bt bf := IFop SA SB tffa tffb bt bf GE.
 
 Definition IFCMPop (a : comparable_type) SA SB tffa tffb
-           (bt : instruction self_type tffa SA SB) (bf : instruction self_type tffb SA SB)
+           (bt : instruction_seq self_type tffa SA SB) (bf : instruction_seq self_type tffb SA SB)
            (op : instruction self_type Datatypes.false (int ::: SA) (bool ::: SA)) :
   instruction self_type (tffa && tffb) (a ::: a ::: SA) SB :=
-  COMPARE ;; op ;; IF bt bf.
+  Instruction_seq (COMPARE ;; op ;; wrap_IF bt bf).
 
 Definition IFCMPEQ {a SA SB tffa tffb} bt bf := IFCMPop a SA SB tffa tffb bt bf EQ.
 Definition IFCMPNEQ {a SA SB tffa tffb} bt bf := IFCMPop a SA SB tffa tffb bt bf NEQ.
@@ -60,12 +66,14 @@ Definition IFCMPGT {a SA SB tffa tffb} bt bf := IFCMPop a SA SB tffa tffb bt bf 
 Definition IFCMPLE {a SA SB tffa tffb} bt bf := IFCMPop a SA SB tffa tffb bt bf LE.
 Definition IFCMPGE {a SA SB tffa tffb} bt bf := IFCMPop a SA SB tffa tffb bt bf GE.
 
-Definition FAIL {SA SB} : instruction self_type Datatypes.true SA SB := UNIT ;; FAILWITH.
+Definition FAIL {SA SB} : instruction self_type Datatypes.true SA SB :=
+  Instruction_seq { UNIT; FAILWITH }.
 
-Definition ASSERT {S} : instruction self_type Datatypes.false (bool ::: S) S := (IF_ IF_bool) NOOP FAIL.
+Definition ASSERT {S} : instruction self_type Datatypes.false (bool ::: S) S :=
+  IF_ IF_bool {} { FAIL }.
 
 Definition ASSERT_op S (op : instruction self_type Datatypes.false (int ::: S) (bool ::: S)) : instruction self_type Datatypes.false (int ::: S) S :=
-  IFop _ _ _ _ NOOP FAIL op.
+  IFop _ _ _ _ {} { FAIL } op.
 
 Definition ASSERT_EQ {S} := ASSERT_op S EQ.
 Definition ASSERT_NEQ {S} := ASSERT_op S NEQ.
@@ -75,7 +83,8 @@ Definition ASSERT_LE {S} := ASSERT_op S LE.
 Definition ASSERT_GE {S} := ASSERT_op S GE.
 
 Definition ASSERT_CMPop (a : comparable_type) S (op : instruction self_type Datatypes.false (int ::: S) (bool ::: S))
-  : instruction self_type Datatypes.false (a ::: a ::: S) S := IFCMPop _ _ _ _ _ NOOP FAIL op.
+  : instruction self_type Datatypes.false (a ::: a ::: S) S :=
+  IFCMPop _ _ _ _ _ {} { FAIL } op.
 
 Definition ASSERT_CMPEQ {a S} := ASSERT_CMPop a S EQ.
 Definition ASSERT_CMPNEQ {a S} := ASSERT_CMPop a S NEQ.
@@ -85,15 +94,16 @@ Definition ASSERT_CMPLE {a S} := ASSERT_CMPop a S LE.
 Definition ASSERT_CMPGE {a S} := ASSERT_CMPop a S GE.
 
 Definition ASSERT_NONE {a S} : instruction self_type Datatypes.false (option a ::: S) S :=
-  IF_NONE NOOP FAIL.
+  IF_NONE {} { FAIL }.
 
 Definition ASSERT_SOME {a S} : instruction self_type Datatypes.false (option a ::: S) (a ::: S) :=
-  IF_NONE FAIL NOOP.
+  IF_NONE { FAIL } {}.
 
 Definition ASSERT_LEFT {a b an bn S} : instruction self_type Datatypes.false (or a an b bn ::: S) (a ::: S) :=
-  IF_LEFT NOOP FAIL.
+  IF_LEFT {} { FAIL }.
+
 Definition ASSERT_RIGHT {a b an bn S} : instruction self_type Datatypes.false (or a an b bn ::: S) (b ::: S) :=
-  IF_LEFT FAIL NOOP.
+  IF_LEFT { FAIL } {}.
 
 Definition DROP1 {a SA} : instruction self_type Datatypes.false (a ::: SA) SA :=
   DROP (A := a ::: nil) 1 eq_refl.
@@ -110,10 +120,10 @@ Definition DIIIIP {a b c d SA SB} code :
   DIP (A := (a ::: b ::: c ::: d ::: nil)) 4 eq_refl code.
 
 Definition DUUP {a b S} : instruction self_type Datatypes.false (a ::: b ::: S) (b ::: a ::: b ::: S) :=
-  DIP1 DUP ;; SWAP.
+  Instruction_seq { DIP1 { DUP }; SWAP }.
 
 Definition DUPn {A b C} n (H : length A = n) : instruction self_type Datatypes.false (A +++ b ::: C) (b ::: A +++ b ::: C) :=
-  DIG n H ;; DUP ;; DIP1 (DUG n H).
+  Instruction_seq { DIG n H; DUP; DIP1 { DUG n H }}.
 
 Definition DUUUP {a b c S} : instruction self_type Datatypes.false (a ::: b ::: c ::: S) (c ::: a ::: b ::: c ::: S) :=
   DUPn (A := a ::: b ::: nil) 2 eq_refl.
@@ -124,41 +134,45 @@ Definition DUUUUP {a b c d S} : instruction self_type Datatypes.false (a ::: b :
 (* Missing: PAPPAIIR and such *)
 
 Definition UNPAIR {a b S} : instruction self_type Datatypes.false (pair a b ::: S) (a ::: b ::: S) :=
-  DUP ;; CAR ;; DIP1 CDR.
+  Instruction_seq { DUP; CAR; DIP1 (instruction_wrap CDR) }%michelson.
 
 Definition CAAR {a b c S} : instruction self_type Datatypes.false (pair (pair a b) c ::: S) (a ::: S) :=
-  CAR ;; CAR.
+  Instruction_seq { CAR; CAR }.
 
 Definition CADR {a b c S} : instruction self_type Datatypes.false (pair (pair a b) c ::: S) (b ::: S) :=
-  CAR ;; CDR.
+  Instruction_seq { CAR; CDR}.
 
 Definition CDAR {a b c S} : instruction self_type Datatypes.false (pair a (pair b c) ::: S) (b ::: S) :=
-  CDR ;; CAR.
+  Instruction_seq { CDR; CAR}.
 
 Definition CDDR {a b c S} : instruction self_type Datatypes.false (pair a (pair b c) ::: S) (c ::: S) :=
-  CDR ;; CDR.
+  Instruction_seq { CDR; CDR}.
 
-Definition IF_SOME {a SA SB tffa tffb} (bt : instruction self_type tffa _ _) (bf : instruction self_type tffb _ _) : instruction self_type _ (option a ::: SA) SB :=
+Definition IF_SOME {a SA SB tffa tffb} (bt : instruction_seq self_type tffa _ _) (bf : instruction_seq self_type tffb _ _) : instruction self_type _ (option a ::: SA) SB :=
   IF_NONE bf bt.
 
-Definition IF_RIGHT {a an b bn SA SB tffa tffb} (bt : instruction self_type tffa _ _) (bf : instruction self_type tffb _ _) : instruction self_type _ (or a an b bn ::: SA) SB :=
+Definition IF_RIGHT {a an b bn SA SB tffa tffb} (bt : instruction_seq self_type tffa _ _) (bf : instruction_seq self_type tffb _ _) : instruction self_type _ (or a an b bn ::: SA) SB :=
   IF_LEFT bf bt.
 
 Definition SET_CAR {a b S} : instruction self_type Datatypes.false (pair a b ::: a ::: S) (pair a b ::: S) :=
-  CDR ;; SWAP ;; PAIR.
+  Instruction_seq { CDR; SWAP; PAIR }%michelson.
 
 Definition SET_CDR {a b S} : instruction self_type Datatypes.false (pair a b ::: b ::: S) (pair a b ::: S) :=
-  CAR ;; PAIR.
+  Instruction_seq { CAR; PAIR }%michelson.
 
-Definition MAP_CAR {a1 a2 b S} (code : instruction self_type Datatypes.false (a1 ::: S) (a2 ::: S)) :
+Definition MAP_CAR {a1 a2 b S} (code : instruction_seq self_type Datatypes.false (a1 ::: S) (a2 ::: S)) :
   instruction self_type Datatypes.false (pair a1 b ::: S) (pair a2 b ::: S) :=
-  DUP ;; CDR ;; DIP1 (CAR ;; code) ;; SWAP ;; PAIR.
+  Instruction_seq { DUP; CDR; DIP1 { CAR; Instruction_seq code}; SWAP; PAIR }%michelson.
 
-Definition MAP_CDR {a b1 b2 S} (code : instruction self_type Datatypes.false (b1 ::: pair a b1 ::: S) (b2 ::: pair a b1 ::: S)) :
+Definition MAP_CDR {a b1 b2 S} (code : instruction_seq self_type Datatypes.false (b1 ::: pair a b1 ::: S) (b2 ::: pair a b1 ::: S)) :
   instruction self_type Datatypes.false (pair a b1 ::: S) (pair a b2 ::: S) :=
-  DUP ;; CDR ;; code ;; SWAP ;; CAR ;; PAIR.
+  Instruction_seq { DUP; CDR; Instruction_seq code; SWAP; CAR; PAIR}%michelson.
 
+Definition UNPAPAIR {a b c S} : instruction self_type Datatypes.false (pair a (pair b c) :: S) (a ::: b ::: c ::: S) :=
+  Instruction_seq { UNPAIR; DIP1 { UNPAIR } }.
 
-Definition UNPAPAIR {a b c S} : instruction self_type Datatypes.false (pair a (pair b c) :: S) (a ::: b ::: c ::: S) := UNPAIR ;; DIP1 UNPAIR.
-Definition PAPAIR {a b c S} : instruction self_type Datatypes.false (a ::: b ::: c ::: S) (pair a (pair b c) :: S) := DIP1 PAIR;; PAIR.
+Definition PAPAIR {a b c S} : instruction self_type Datatypes.false (a ::: b ::: c ::: S) (pair a (pair b c) :: S) :=
+  Instruction_seq { DIP1 { PAIR }; PAIR }.
+
 End macros.
+
